src/basic/FStarC.Errors.Codes.fsti
@@ -402,6 +402,8 @@ type error_code =
   | Warning_CustardNoPublicDefinitions
   | Error_CustardMonoExternal
   | Warning_CustardGeneratedNameInInterface
+  | Error_CustardBadLift
+  | Error_CustardDanglingReference
   | Error_AmbiguousName
 
 type error_setting = error_code & error_flag & int
